moved relations out of submodules, and derived DecOpt instances

src/PlutusIR/Analysis/BoundVars.v
@@ -11,6 +11,7 @@ Local Open Scope string_scope.
 
 From PlutusCert Require Import
   Util
+  Util.List
   PlutusIR
   PlutusIR.Folds
   .
@@ -19,39 +20,40 @@ Require Import Utf8_core.
 
 Import NamedTerm.
 
-Module Ty.
 
-  Inductive appears_bound_in (X: string) : Ty -> Prop :=
-    | ABI_TyFun1 : forall T1 T2,
-        appears_bound_in X T1 ->
-        appears_bound_in X (Ty_Fun T1 T2)
-    | ABI_TyFun2 : forall T1 T2,
-        appears_bound_in X T2 ->
-        appears_bound_in X (Ty_Fun T1 T2)
-    | ABI_TyIFix1 : forall F T,
-        appears_bound_in X F ->
-        appears_bound_in X (Ty_IFix F T)
-    | ABI_TyIFix2 : forall F T,
-        appears_bound_in X T ->
-        appears_bound_in X (Ty_IFix F T)
-    | ABI_TyForall1 : forall K T,
-        appears_bound_in X (Ty_Forall X K T)
-    | ABI_TyForall2 : forall Y K T,
-        X <> Y ->
-        appears_bound_in Y T ->
-        appears_bound_in X (Ty_Forall Y K T)
-    | ABI_TyLam1 : forall K T,
-        appears_bound_in X (Ty_Lam X K T)
-    | ABI_TyLam2 : forall Y K T,
-        X <> Y ->
-        appears_bound_in Y T ->
-        appears_bound_in X (Ty_Lam Y K T)
-    | ABI_TyApp1 : forall T1 T2,
-        appears_bound_in X T1 ->
-        appears_bound_in X (Ty_App T1 T2)
-    | ABI_TyApp2 : forall T1 T2,
-        appears_bound_in X T2 ->
-        appears_bound_in X (Ty_App T1 T2).
+Inductive appears_bound_in_ty (X : string) : Ty -> Prop :=
+  | ABI_Ty_TyFun1 : forall T1 T2,
+      appears_bound_in_ty X T1 ->
+      appears_bound_in_ty X (Ty_Fun T1 T2)
+  | ABI_Ty_TyFun2 : forall T1 T2,
+      appears_bound_in_ty X T2 ->
+      appears_bound_in_ty X (Ty_Fun T1 T2)
+  | ABI_Ty_TyIFix1 : forall F T,
+      appears_bound_in_ty X F ->
+      appears_bound_in_ty X (Ty_IFix F T)
+  | ABI_Ty_TyIFix2 : forall F T,
+      appears_bound_in_ty X T ->
+      appears_bound_in_ty X (Ty_IFix F T)
+  | ABI_Ty_TyForall1 : forall K T,
+      appears_bound_in_ty X (Ty_Forall X K T)
+  | ABI_Ty_TyForall2 : forall Y K T,
+      X <> Y ->
+      appears_bound_in_ty Y T ->
+      appears_bound_in_ty X (Ty_Forall Y K T)
+  | ABI_Ty_TyLam1 : forall K T,
+      appears_bound_in_ty X (Ty_Lam X K T)
+  | ABI_Ty_TyLam2 : forall Y K T,
+      X <> Y ->
+      appears_bound_in_ty Y T ->
+      appears_bound_in_ty X (Ty_Lam Y K T)
+  | ABI_Ty_TyApp1 : forall T1 T2,
+      appears_bound_in_ty X T1 ->
+      appears_bound_in_ty X (Ty_App T1 T2)
+  | ABI_Ty_TyApp2 : forall T1 T2,
+      appears_bound_in_ty X T2 ->
+      appears_bound_in_ty X (Ty_App T1 T2).
+
+Module Ty.
 
   Section btv.
     Context
@@ -80,125 +82,123 @@ Module Ty.
 
 End Ty.
 
-Module Term.
 
-  Definition bv_constructor (c : constructor) : string :=
-    match c with
-    | Constructor (VarDecl x _) _ => x
-    end.
 
-  Inductive appears_bound_in (x : string) : Term -> Prop :=
-    | ABI_LamAbs1 : forall T t,
-        appears_bound_in x (LamAbs x T t)
-    | ABI_LamAbs2 : forall y T t,
-        x <> y ->
-        appears_bound_in x t ->
-        appears_bound_in x (LamAbs y T t)
-    | ABI_Apply1 : forall t1 t2,
-        appears_bound_in x t1 ->
-        appears_bound_in x (Apply t1 t2)
-    | ABI_Apply2 : forall t1 t2,
-        appears_bound_in x t2 ->
-        appears_bound_in x (Apply t1 t2)
-    | ABI_TyAbs : forall X K t,
-        appears_bound_in x t ->
-        appears_bound_in x (TyAbs X K t)
-    | ABI_TyInst : forall t T,
-        appears_bound_in x t ->
-        appears_bound_in x (TyInst t T)
-    | ABI_IWrap : forall F T t,
-        appears_bound_in x t ->
-        appears_bound_in x (IWrap F T t)
-    | ABI_Unwrap : forall t,
-        appears_bound_in x t ->
-        appears_bound_in x (Unwrap t)
-    | ABI_Let_Nil : forall recty t0,
-        appears_bound_in x t0 ->
-        appears_bound_in x (Let recty nil t0)
-    | ABI_Let_Cons : forall recty b bs t0,
-        appears_bound_in x (Let recty bs t0) ->
-        appears_bound_in x (Let recty (b :: bs) t0)
-    | ABI_Let_TermBind1 : forall recty stricty T t bs t0,
-        appears_bound_in x (Let recty (TermBind stricty (VarDecl x T) t :: bs) t0)
-    | ABI_Let_TermBind2 : forall recty stricty y T t bs t0,
-        appears_bound_in x t ->
-        appears_bound_in x (Let recty (TermBind stricty (VarDecl y T) t :: bs) t0)
-    | ABI_Let_DatatypeBind : forall recty XK YKs mfunc cs t0 bs,
-        In x (mfunc :: map bv_constructor cs) ->
-        appears_bound_in x (Let recty (DatatypeBind (Datatype XK YKs mfunc cs) :: bs) t0)
-    .
+(* Monomorphic alternative for `map bvc`, for dec procedure generation *)
+Fixpoint bv_constructors (cs : list constructor) : list string :=
+  match cs with
+  | [] => []
+  | Constructor (VarDecl x _) _ :: cs' => x :: bv_constructors cs'
+  end.
 
-End Term.
+Inductive appears_bound_in_tm (x : string) : Term -> Prop :=
+  | ABI_Tm_LamAbs1 : forall T t,
+      appears_bound_in_tm x (LamAbs x T t)
+  | ABI_Tm_LamAbs2 : forall y T t,
+      x <> y ->
+      appears_bound_in_tm x t ->
+      appears_bound_in_tm x (LamAbs y T t)
+  | ABI_Tm_Apply1 : forall t1 t2,
+      appears_bound_in_tm x t1 ->
+      appears_bound_in_tm x (Apply t1 t2)
+  | ABI_Tm_Apply2 : forall t1 t2,
+      appears_bound_in_tm x t2 ->
+      appears_bound_in_tm x (Apply t1 t2)
+  | ABI_Tm_TyAbs : forall X K t,
+      appears_bound_in_tm x t ->
+      appears_bound_in_tm x (TyAbs X K t)
+  | ABI_Tm_TyInst : forall t T,
+      appears_bound_in_tm x t ->
+      appears_bound_in_tm x (TyInst t T)
+  | ABI_Tm_IWrap : forall F T t,
+      appears_bound_in_tm x t ->
+      appears_bound_in_tm x (IWrap F T t)
+  | ABI_Tm_Unwrap : forall t,
+      appears_bound_in_tm x t ->
+      appears_bound_in_tm x (Unwrap t)
+  | ABI_Tm_Let_Nil : forall recty t0,
+      appears_bound_in_tm x t0 ->
+      appears_bound_in_tm x (Let recty nil t0)
+  | ABI_Tm_Let_Cons : forall recty b bs t0,
+      appears_bound_in_tm x (Let recty bs t0) ->
+      appears_bound_in_tm x (Let recty (b :: bs) t0)
+  | ABI_Tm_Let_TermBind1 : forall recty stricty T t bs t0,
+      appears_bound_in_tm x (Let recty (TermBind stricty (VarDecl x T) t :: bs) t0)
+  | ABI_Tm_Let_TermBind2 : forall recty stricty y T t bs t0,
+      x <> y ->
+      appears_bound_in_tm x t ->
+      appears_bound_in_tm x (Let recty (TermBind stricty (VarDecl y T) t :: bs) t0)
+  | ABI_Tm_Let_DatatypeBind : forall recty XK YKs mfunc cs t0 bs,
+      NameIn x (mfunc :: bv_constructors cs) ->
+      appears_bound_in_tm x (Let recty (DatatypeBind (Datatype XK YKs mfunc cs) :: bs) t0) 
+      .
 
-Module Annotation.
+Inductive appears_bound_in_ann (X : string) : Term -> Prop :=
+  | ABI_Ann_LamAbs1 : forall x T t,
+      appears_bound_in_ty X T ->
+      appears_bound_in_ann X (LamAbs x T t)
+  | ABI_Ann_LamAbs : forall x T t,
+      appears_bound_in_ann X t ->
+      appears_bound_in_ann X (LamAbs x T t)
+  | ABI_Ann_Apply1 : forall t1 t2,
+      appears_bound_in_ann X t1 ->
+      appears_bound_in_ann X (Apply t1 t2)
+  | ABI_Ann_Apply2 : forall t1 t2,
+      appears_bound_in_ann X t2 ->
+      appears_bound_in_ann X (Apply t1 t2)
+  | ABI_Ann_TyAbs1 : forall K t,
+      appears_bound_in_ann X (TyAbs X K t)
+  | ABI_Ann_TyAbs2 : forall Y K t,
+      X <> Y ->
+      appears_bound_in_ann X t ->
+      appears_bound_in_ann X (TyAbs Y K t)
+  | ABI_Ann_TyInst1 : forall t T,
+      appears_bound_in_ann X t ->
+      appears_bound_in_ann X (TyInst t T)
+  | ABI_Ann_TyInst2 : forall t T,
+      appears_bound_in_ty X T ->
+      appears_bound_in_ann X (TyInst t T)
+  | ABI_Ann_IWrap1 : forall F T t,
+      appears_bound_in_ty X F ->
+      appears_bound_in_ann X (IWrap F T t)
+  | ABI_Ann_IWrap2 : forall F T t,
+      appears_bound_in_ty X T ->
+      appears_bound_in_ann X (IWrap F T t)
+  | ABI_Ann_IWrap3 : forall F T t,
+      appears_bound_in_ann X t ->
+      appears_bound_in_ann X (IWrap F T t)
+  | ABI_Ann_Unwrap : forall t,
+      appears_bound_in_ann X t ->
+      appears_bound_in_ann X (Unwrap t)
+  | ABI_Ann_Error : forall T,
+      appears_bound_in_ty X T ->
+      appears_bound_in_ann X (Error T)
+  | ABI_Ann_Let_Nil : forall recty t0,
+      appears_bound_in_ann X t0 ->
+      appears_bound_in_ann X (Let recty nil t0)
+  | ABI_Ann_Let_Cons : forall recty b bs t0,
+      appears_bound_in_ann X (Let recty bs t0) ->
+        appears_bound_in_ann X (Let recty (b :: bs) t0)
+  | ABI_Ann_Let_TermBind1 : forall recty stricty x T t bs t0,
+      appears_bound_in_ty X T ->
+      appears_bound_in_ann X (Let recty (TermBind stricty (VarDecl x T) t :: bs) t0)
+  | ABI_Ann_Let_TermBind2 : forall recty stricty y T t bs t0,
+      appears_bound_in_ann X t ->
+      appears_bound_in_ann X (Let recty (TermBind stricty (VarDecl y T) t :: bs) t0)
+  | ABI_Ann_Let_TypeBind1 : forall recty K T bs t0,
+      appears_bound_in_ann X (Let recty (TypeBind (TyVarDecl X K) T :: bs) t0)
+  | ABI_Ann_Let_TypeBind2 : forall recty Y K T bs t0,
+      X <> Y ->
+      appears_bound_in_ty X T ->
+      appears_bound_in_ann X (Let recty (TypeBind (TyVarDecl Y K) T :: bs) t0)
+  | ABI_Ann_Let_DatatypeBind : forall recty K YKs mfunc cs t0 bs,
+      appears_bound_in_ann X (Let recty (DatatypeBind (Datatype (TyVarDecl X K) YKs mfunc cs) :: bs) t0) 
+  .
 
-  Inductive appears_bound_in (X : string) : Term -> Prop :=
-    | ABI_LamAbs1 : forall x T t,
-        Ty.appears_bound_in X T ->
-        appears_bound_in X (LamAbs x T t)
-    | ABI_LamAbs : forall x T t,
-        appears_bound_in X t ->
-        appears_bound_in X (LamAbs x T t)
-    | ABI_Apply1 : forall t1 t2,
-        appears_bound_in X t1 ->
-        appears_bound_in X (Apply t1 t2)
-    | ABI_Apply2 : forall t1 t2,
-        appears_bound_in X t2 ->
-        appears_bound_in X (Apply t1 t2)
-    | ABI_TyAbs1 : forall K t,
-        appears_bound_in X (TyAbs X K t)
-    | ABI_TyAbs2 : forall Y K t,
-        X <> Y ->
-        appears_bound_in X t ->
-        appears_bound_in X (TyAbs Y K t)
-    | ABI_TyInst1 : forall t T,
-        appears_bound_in X t ->
-        appears_bound_in X (TyInst t T)
-    | ABI_TyInst2 : forall t T,
-        Ty.appears_bound_in X T ->
-        appears_bound_in X (TyInst t T)
-    | ABI_IWrap1 : forall F T t,
-        Ty.appears_bound_in X F ->
-        appears_bound_in X (IWrap F T t)
-    | ABI_IWrap2 : forall F T t,
-        Ty.appears_bound_in X T ->
-        appears_bound_in X (IWrap F T t)
-    | ABI_IWrap3 : forall F T t,
-        appears_bound_in X t ->
-        appears_bound_in X (IWrap F T t)
-    | ABI_Unwrap : forall t,
-        appears_bound_in X t ->
-        appears_bound_in X (Unwrap t)
-    | ABI_Error : forall T,
-        Ty.appears_bound_in X T ->
-        appears_bound_in X (Error T)
-    | ABI_Let_Nil : forall recty t0,
-        appears_bound_in X t0 ->
-        appears_bound_in X (Let recty nil t0)
-    | ABI_Let_Cons : forall recty b bs t0,
-        appears_bound_in X (Let recty bs t0) ->
-        appears_bound_in X (Let recty (b :: bs) t0)
-    | ABI_Let_TermBind1 : forall recty stricty x T t bs t0,
-        Ty.appears_bound_in X T ->
-        appears_bound_in X (Let recty (TermBind stricty (VarDecl x T) t :: bs) t0)
-    | ABI_Let_TermBind2 : forall recty stricty y T t bs t0,
-        appears_bound_in X t ->
-        appears_bound_in X (Let recty (TermBind stricty (VarDecl y T) t :: bs) t0)
-    | ABI_Let_TypeBind1 : forall recty K T bs t0,
-        appears_bound_in X (Let recty (TypeBind (TyVarDecl X K) T :: bs) t0)
-    | ABI_Let_TypeBind2 : forall recty Y K T bs t0,
-        Ty.appears_bound_in X T ->
-        appears_bound_in X (Let recty (TypeBind (TyVarDecl Y K) T :: bs) t0)
-    | ABI_Let_DatatypeBind : forall recty K YKs mfunc cs t0 bs,
-        appears_bound_in X (Let recty (DatatypeBind (Datatype (TyVarDecl X K) YKs mfunc cs) :: bs) t0)
-    .
-
-End Annotation.
-
-#[export] Hint Constructors
-  Ty.appears_bound_in
-  Term.appears_bound_in
-  Annotation.appears_bound_in
+#[export] Hint Constructors 
+  appears_bound_in_ty
+  appears_bound_in_tm
+  appears_bound_in_ann
   : core.
 
 
@@ -307,13 +307,11 @@ with btv_binding (b : binding') : list tyvar := match b with
 
 End BoundVars.
 
-Import BoundVars.Term.
+Definition P_Term (t : Term) : Prop := Forall (fun v => appears_bound_in_tm v t) (bound_vars t).
+Definition P_Binding (b : Binding) := Forall (fun v => forall t bs recty, appears_bound_in_tm v (Let recty (b :: bs) t)) (bound_vars_binding b).
 
-Definition P_Term (t : Term) : Prop := Forall (fun v => appears_bound_in v t) (bound_vars t).
-Definition P_Binding (b : Binding) := Forall (fun v => forall t bs recty, appears_bound_in v (Let recty (b :: bs) t)) (bound_vars_binding b).
-
-Lemma bound_vars_appears_bound_in : (forall t, P_Term t) /\ (forall b, P_Binding b).
-Proof with eauto using appears_bound_in.
+Lemma bound_vars_appears_bound_in_tm : (forall t, P_Term t) /\ (forall b, P_Binding b).
+Proof with eauto using appears_bound_in_tm.
   apply Term__multind with (P := P_Term) (Q := P_Binding).
   all: unfold P_Term...
   - intros.
@@ -336,12 +334,12 @@ Proof with eauto using appears_bound_in.
              apply ForallP_Forall in H.
              apply IHbs in H.
              eapply Forall_impl.
-             intros b. apply ABI_Let_Cons.
+             intros b. apply ABI_Tm_Let_Cons.
              auto.
 
     + unfold P_Term in *.
-      eapply Forall_impl with (P := fun v => appears_bound_in v t)...
-      eauto using appears_bound_in.
+      eapply Forall_impl with (P := fun v => appears_bound_in_tm v t)...
+      eauto using appears_bound_in_tm.
       intros.
       induction bs...
       apply ForallP_Forall in H.
@@ -355,26 +353,26 @@ Proof with eauto using appears_bound_in.
     eauto.
   - intros.
     eapply Forall_cons...
-    eapply Forall_impl with (P := fun a => appears_bound_in a t0)...
+    eapply Forall_impl with (P := fun a => appears_bound_in_tm a t0)...
     intros.
       destruct (string_dec a s).
-      * subst. apply ABI_LamAbs1.
-      * apply ABI_LamAbs2...
+      * subst. apply ABI_Tm_LamAbs1.
+      * apply ABI_Tm_LamAbs2...
 
-  (* Common pattern: only need to prove an implication using a ABI rule *)
+  (* Common pattern: only need to prove an implication using a ABI_Tm rule *)
   Ltac tac rule :=
     intros; eapply Forall_impl; [intros a; apply rule | auto].
 
   - intros.
     apply Forall_app. split.
-      + tac ABI_Apply1.
-      + tac ABI_Apply2.
+      + tac ABI_Tm_Apply1.
+      + tac ABI_Tm_Apply2.
   - intros. cbv. auto.
   - intros. cbv. auto.
-  - tac ABI_TyInst.
+  - tac ABI_Tm_TyInst.
   - intros. cbv. auto.
-  - tac ABI_IWrap.
-  - tac ABI_Unwrap.
+  - tac ABI_Tm_IWrap.
+  - tac ABI_Tm_Unwrap.
   - intros.
     unfold P_Binding.
     intros.
@@ -382,9 +380,8 @@ Proof with eauto using appears_bound_in.
     destruct v.
     eapply Forall_cons.
       + intros...
-      + intros. eapply Forall_impl with (P := fun v => appears_bound_in v t).
-        1: { intros. apply ABI_Let_TermBind2... }
-        auto.
+      + intros. eapply Forall_impl with (P := fun v => appears_bound_in_tm v t)...
+        intros. destruct (string_dec a s0); subst...
   - unfold P_Binding.
     intros.
     cbv...
@@ -393,13 +390,17 @@ Proof with eauto using appears_bound_in.
     destruct dtd.
     apply Forall_cons.
     + intros.
-      apply ABI_Let_DatatypeBind.
+      apply ABI_Tm_Let_DatatypeBind.
       constructor...
     + apply Forall_forall.
       intros.
-      apply ABI_Let_DatatypeBind.
+      apply ABI_Tm_Let_DatatypeBind.
+      apply NameIn_In_string_equal.
       apply in_cons.
-      assumption.
+      induction l0...
+      destruct a.
+      destruct v.
+      induction H; subst; simpl...
 Qed.
 
 Inductive decide {a : Type} (P : a -> Type) (x : a) :=
