src/PlutusIR/Analysis/BoundVars/DecOpt.v
@@ -1,0 +1,51 @@
+From PlutusCert Require Import 
+  Util.List
+  PlutusIR
+  PlutusIR.Analysis.BoundVars.
+From QuickChick Require Import QuickChick.
+
+
+
+(* appears_bound_in_ty *)
+
+QCDerive DecOpt for (appears_bound_in_ty x ty).
+
+Instance appears_bound_in_ty_DecOpt_sound x ty: DecOptSoundPos (appears_bound_in_ty x ty).
+Proof. (* derive_sound. Qed. *) idtac "Admitted: appears_bound_in_ty_DecOpt_sound". Admitted.
+
+Instance appears_bound_in_ty_DecOpt_complete x ty: DecOptCompletePos (appears_bound_in_ty x ty).
+Proof. (* derive_complete. Qed. *) idtac "Admitted: appears_bound_in_ty_DecOpt_complete". Admitted.
+
+Instance appears_bound_in_ty_DecOpt_mono x ty: DecOptSizeMonotonic (appears_bound_in_ty x ty).
+Proof. (* derive_mon. Qed. *) idtac "Admitted: appears_bound_in_ty_DecOpt_mon". Admitted.
+
+
+
+
+(* appears_bound_in_tm *)
+
+QCDerive DecOpt for (appears_bound_in_tm x tm).
+
+Instance appears_bound_in_tm_DecOpt_sound x tm: DecOptSoundPos (appears_bound_in_tm x tm).
+Proof. (* derive_sound. Qed. *) idtac "Admitted: appears_bound_in_tm_DecOpt_sound". Admitted.
+
+Instance appears_bound_in_tm_DecOpt_complete x tm: DecOptCompletePos (appears_bound_in_tm x tm).
+Proof. (* derive_complete. Qed. *) idtac "Admitted: appears_bound_in_tm_DecOpt_complete". Admitted.
+
+Instance appears_bound_in_tm_DecOpt_mon x tm: DecOptSizeMonotonic (appears_bound_in_tm x tm).
+Proof. (* derive_mon. Qed. *) idtac "Admitted: appears_bound_in_tm_DecOpt_mon". Admitted.
+
+
+
+(* appears_bound_in_ann *)
+
+QCDerive DecOpt for (appears_bound_in_ann x ann).
+
+Instance appears_bound_in_ann_DecOpt_sound x ann: DecOptSoundPos (appears_bound_in_ann x ann).
+Proof. (* derive_sound. Qed. *) idtac "Admitted: appears_bound_in_ann_DecOpt_sound". Admitted.
+
+Instance appears_bound_in_ann_DecOpt_complete x ann: DecOptCompletePos (appears_bound_in_ann x ann).
+Proof. (* derive_complete. Qed. *) idtac "Admitted: appears_bound_in_ann_DecOpt_complete". Admitted.
+
+Instance appears_bound_in_ann_DecOpt_mon x ann: DecOptSizeMonotonic (appears_bound_in_ann x ann).
+Proof. (* derive_mon. Qed. *) idtac "Admitted: appears_bound_in_ann_DecOpt_mon". Admitted.
