src/PlutusIR/Transform/LetNonRec/DSP.v
@@ -389,7 +389,7 @@ Proof with (eauto_LR || eauto with DSP_compatibility_lemmas).
             destruct (s =? x)%string eqn:Heqb.
             ++ eapply eqb_eq in Heqb as Heq.
                 subst.
-                assert (Annotation.appears_bound_in x (Let NonRec (TypeBind (TyVarDecl x k) t1 :: bs) t)) by eauto.
+                assert (appears_bound_in_ann x (Let NonRec (TypeBind (TyVarDecl x k) t1 :: bs) t)) by eauto.
                 eapply uniqueness' in H4.
                 rewrite H4 in H1.
                 inversion H4.
@@ -403,7 +403,7 @@ Proof with (eauto_LR || eauto with DSP_compatibility_lemmas).
             destruct (s0 =? x)%string eqn:Heqb.
             ++ eapply eqb_eq in Heqb as Heq.
                 subst.
-                assert (Annotation.appears_bound_in x (Let NonRec (DatatypeBind (Datatype (TyVarDecl x k) l s l0) :: bs) t)) by eauto.
+                assert (appears_bound_in_ann x (Let NonRec (DatatypeBind (Datatype (TyVarDecl x k) l s l0) :: bs) t)) by eauto.
                 eapply uniqueness' in H4.
                 rewrite H4 in H1.
                 inversion H4.
@@ -432,7 +432,7 @@ Proof with (eauto_LR || eauto with DSP_compatibility_lemmas).
             destruct (s =? x)%string eqn:Heqb.
             ++ eapply eqb_eq in Heqb as Heq.
                 subst.
-                assert (Annotation.appears_bound_in x (Let NonRec (TypeBind (TyVarDecl x k) t1 :: bs) t)) by eauto.
+                assert (appears_bound_in_ann x (Let NonRec (TypeBind (TyVarDecl x k) t1 :: bs) t)) by eauto.
                 eapply uniqueness' in H4.
                 rewrite H4 in H1.
                 inversion H4.
@@ -446,7 +446,7 @@ Proof with (eauto_LR || eauto with DSP_compatibility_lemmas).
             destruct (s0 =? x)%string eqn:Heqb.
             ++ eapply eqb_eq in Heqb as Heq.
                 subst.
-                assert (Annotation.appears_bound_in x (Let NonRec (DatatypeBind (Datatype (TyVarDecl x k) l s l0) :: bs) t)) by eauto.
+                assert (appears_bound_in_ann x (Let NonRec (DatatypeBind (Datatype (TyVarDecl x k) l s l0) :: bs) t)) by eauto.
                 eapply uniqueness' in H4.
                 rewrite H4 in H1.
                 inversion H4.
